src/Rdf.v
@@ -210,9 +210,11 @@ Section Rdf.
              apply: perm_trans peq_can peq.
       Qed.
 
-      Lemma perm_eq_relab_uniq g1 g2 mu : perm_eq (relabeling_seq_triple mu g1) g2 -> perm_eq (relabeling_seq_triple mu g1) g2 /\ uniq (relabeling_seq_triple mu g1).
+      Lemma perm_eq_relab_uniq_ts ts1 ts2 mu (u2 : uniq ts2) : perm_eq (relabeling_seq_triple mu ts1) ts2 -> perm_eq (relabeling_seq_triple mu ts1) ts2 /\ uniq (relabeling_seq_triple mu ts1).
       Proof. by move=> peq; rewrite (perm_uniq peq) peq. Qed.
 
+      Lemma perm_eq_relab_uniq g1 g2 mu : perm_eq (relabeling_seq_triple mu g1) g2 -> perm_eq (relabeling_seq_triple mu g1) g2 /\ uniq (relabeling_seq_triple mu g1).
+      Proof. by apply perm_eq_relab_uniq_ts. Qed.
 
       Lemma relabeling_triple_comp_map (B1 B2 B3 : eqType) (g : rdf_graph I B1 L) (mu12 : B1 -> B2) (mu23 : B2 -> B3) :
         [seq relabeling_triple mu23 i | i <- relabeling_seq_triple mu12 g] =
@@ -706,14 +708,19 @@ Section Rdf.
         by apply triple_inj=> /=; apply (relabeling_term_inj_terms mu_inj)=> //.
     Qed.
 
-    Lemma map_comp_in_id g (mu nu: B -> B) :
-      [seq (nu \o mu) i | i <- get_b g] = get_b g ->
-        {in (get_b g), nu \o mu =1 id}.
-    Proof. elim: (get_b g)=> [| h t IHtl]; first by move=> _ x; rewrite in_nil //.
+    Lemma map_comp_in_id_ts ts (mu nu: B -> B) :
+      [seq (nu \o mu) i | i <- get_bts ts] = get_bts ts ->
+        {in (get_bts ts), nu \o mu =1 id}.
+    Proof. elim: (get_bts ts)=> [| h t IHtl]; first by move=> _ x; rewrite in_nil //.
            move=> [heq teq] x; rewrite in_cons; case e: (x == h)=> /=.
            + by move: e=> /eqP ->; rewrite heq.
            + apply IHtl; apply teq.
     Qed.
+
+    Lemma map_comp_in_id g (mu nu: B -> B) :
+      [seq (nu \o mu) i | i <- get_b g] = get_b g ->
+        {in (get_b g), nu \o mu =1 id}.
+    Proof. apply map_comp_in_id_ts. Qed.
 
     Lemma bterm_eq_mem_get_b (b: B) g :
       (@Bnode I B L b) \in terms g ->
@@ -893,63 +900,90 @@ Section Rdf.
 
       Section eqb_rdf_perm_eq.
         (* TODO find a place for these lemmas *)
-        Lemma eqb_rdf_terms g1 g2 :
-          eqb_rdf g1 g2 -> perm_eq (terms g1) (terms g2).
+
+        Lemma peq_terms ts1 ts2 :
+          perm_eq ts1 ts2 -> perm_eq (terms_ts ts1) (terms_ts ts2).
         Proof. rewrite /eqb_rdf/terms=> peq.
                by rewrite perm_undup //; apply perm_mem; rewrite perm_flatten //; apply: perm_map peq.
         Qed.
 
-        Lemma eqb_rdf_bnodes g1 g2 :
-          eqb_rdf g1 g2 -> perm_eq (bnodes g1) (bnodes g2).
-        Proof. move=> /eqb_rdf_terms eqb.
+        Lemma eqb_rdf_terms g1 g2 :
+          eqb_rdf g1 g2 -> perm_eq (terms g1) (terms g2).
+        Proof. by apply peq_terms. Qed.
+
+        Lemma peq_bnodes ts1 ts2 :
+          perm_eq ts1 ts2 -> perm_eq (bnodes_ts ts1) (bnodes_ts ts2).
+        Proof. move=> /peq_terms eqb.
                by rewrite /bnodes perm_undup //; apply: perm_mem; apply: perm_filter.
         Qed.
 
+        Lemma eqb_rdf_bnodes g1 g2 :
+          eqb_rdf g1 g2 -> perm_eq (bnodes g1) (bnodes g2).
+        Proof. by apply peq_bnodes. Qed.
+
+        Lemma peq_get_bts ts1 ts2 :
+          perm_eq ts1 ts2 -> perm_eq (get_bts ts1) (get_bts ts2).
+        Proof. by move=> /peq_bnodes eqb ; apply: perm_pmap eqb. Qed.
+
         Lemma eqb_rdf_get_b g1 g2 :
           eqb_rdf g1 g2 -> perm_eq (get_b g1) (get_b g2).
-        Proof. by move=> /eqb_rdf_bnodes eqb ; rewrite /get_b/get_bs; apply: perm_pmap eqb. Qed.
+        Proof. by move=> /peq_bnodes eqb ; apply: perm_pmap eqb. Qed.
+
+        Lemma peq_get_bts_hom ts1 ts2 mu :
+          uniq (relabeling_seq_triple mu ts1) ->
+          perm_eq (relabeling_seq_triple mu ts1) ts2 -> perm_eq (undup (map mu (get_bts ts1))) (get_bts ts2).
+        Proof. by move=> us /peq_get_bts eqb ; rewrite (perm_eq_bnodes_relabel eqb). Qed.
 
         Lemma eqb_rdf_get_b_hom g1 g2 mu us :
           eqb_rdf (@relabeling _ _ mu g1 us) g2 -> perm_eq (undup (map mu (get_b g1))) (get_b g2).
-        Proof.
-          by move=> /eqb_rdf_get_b eqb ; rewrite /get_b/bnodes/relabeling (perm_eq_bnodes_relabel eqb).
-        Qed.
+        Proof. by apply peq_get_bts_hom. Qed.
 
       End eqb_rdf_perm_eq.
 
-      Remark eqiso g1 g2 : eqb_rdf g1 g2 -> iso g1 g2.
+      Remark eqiso_ts ts1 ts2 (u1 : uniq ts1) : perm_eq ts1 ts2 -> iso_ts ts1 ts2.
       Proof.
         exists id.
-        have usid: uniq (relabeling_seq_triple id g1) by rewrite relabeling_seq_triple_id; case g1.
+        have usid: uniq (relabeling_seq_triple id ts1) by rewrite relabeling_seq_triple_id.
         rewrite /is_iso/is_iso_ts usid /is_pre_iso/is_pre_iso_ts map_id relabeling_seq_triple_id /=; apply/andP; split=> //.
-        - exact: eqb_rdf_get_b.
+        - exact: peq_get_bts.
+      Qed.
+
+
+      Remark eqiso g1 g2 : eqb_rdf g1 g2 -> iso g1 g2.
+      Proof. by apply : eqiso_ts (uniq_rdf_graph _). Qed.
+
+      Lemma iso_ts_sym ts1 ts2 (u1 : uniq ts1) (u2 : uniq ts2) : iso_ts ts1 ts2 <-> iso_ts ts2 ts1.
+      Proof.
+        suffices imp h1 h2 : uniq h1 -> iso_ts h1 h2 -> iso_ts h2 h1 by split; exact: imp.
+        move=> uh1; case=> mu /and3P[pre_iso_mu uniq_relab perm_relab].
+        move:(is_pre_iso_ts_inv pre_iso_mu); rewrite /pre_iso/is_pre_iso; move=> [nu [pre_iso_nu /map_comp_in_id_ts/can_bs_can_rtbs nuP]].
+        exists nu.
+        rewrite /is_iso/is_iso_ts pre_iso_nu.
+        suffices peq : perm_eq (relabeling_seq_triple nu h2) h1.
+          by move/(perm_eq_relab_uniq_ts uh1) : peq => [-> ->].
+        move: perm_relab; rewrite perm_sym=> /(perm_map (relabeling_triple nu))=> perm_relab.
+        by apply: perm_trans perm_relab _; rewrite relabeling_triple_map_comp map_id_in //.
       Qed.
 
       Lemma iso_sym g1 g2 : iso g1 g2 <-> iso g2 g1.
-      Proof.
-        suffices imp h1 h2 : iso h1 h2 -> iso h2 h1 by split; exact: imp.
-        case=> mu /and3P[pre_iso_mu uniq_relab perm_relab].
-        move:(is_pre_iso_inv pre_iso_mu); rewrite /pre_iso/is_pre_iso; move=> [nu [pre_iso_nu /map_comp_in_id/can_b_can_rtb nuP]].
-        exists nu.
-        rewrite /is_iso/is_iso_ts pre_iso_nu.
-        have /perm_eq_relab_uniq [-> ->] //: perm_eq (relabeling_seq_triple nu h2) h1.
-        move: perm_relab; rewrite perm_sym=> /(perm_map (relabeling_triple nu))=> perm_relab.
-        apply: perm_trans perm_relab _; rewrite relabeling_triple_map_comp map_id_in //.
-      Qed.
+      Proof. by apply: iso_ts_sym (uniq_rdf_graph _) (uniq_rdf_graph _). Qed.
 
-      Lemma iso_trans g1 g2 g3 : iso g1 g2 -> iso g2 g3 -> iso g1 g3.
+      Lemma iso_ts_trans ts1 ts2 ts3 : iso_ts ts1 ts2 -> iso_ts ts2 ts3 -> iso_ts ts1 ts3.
       Proof. rewrite /iso/is_iso; move=> [mu12 /and3P[pre_iso12 urel12 perm12]] [mu23 /and3P[pre_iso23 urel23 perm23]].
              exists (mu23 \o mu12).
-             suffices ucomp: uniq (relabeling_seq_triple (mu23 \o mu12) g1).
+             suffices ucomp: uniq (relabeling_seq_triple (mu23 \o mu12) ts1).
              apply /and3P; split=> //.
-             + by apply: is_pre_iso_trans pre_iso12 pre_iso23.
-             + by apply : eqb_relabeling_comp perm12 perm23.
+             + by apply: is_pre_iso_ts_trans pre_iso12 pre_iso23.
+             + by apply : perm_eq_comp perm12 perm23.
              + rewrite -relabeling_seq_triple_comp /relabeling_seq_triple.
-               have /eq_uniq -> //: size [seq relabeling_triple mu23 i | i <- [seq relabeling_triple mu12 i | i <- g1]] =
-                             size (relabeling_seq_triple mu23 g2).
+               have /eq_uniq -> //: size [seq relabeling_triple mu23 i | i <- [seq relabeling_triple mu12 i | i <- ts1]] =
+                             size (relabeling_seq_triple mu23 ts2).
                by move: perm12=> /perm_size; rewrite !size_map.
                by apply eq_mem_map; apply perm_mem.
       Qed.
+
+      Lemma iso_trans g1 g2 g3 : iso g1 g2 -> iso g2 g3 -> iso g1 g3.
+      Proof. by apply iso_ts_trans. Qed.
 
       Lemma ts_pre_iso_iso ts mu (urel: uniq (relabeling_seq_triple mu ts)) :
         is_pre_iso_ts ts (relabeling_seq_triple mu ts) mu ->
@@ -973,6 +1007,16 @@ Section Rdf.
           have isog1k1 : iso g1 (M g1). by apply iso_output.
           have isog2k2 : iso (M g2) g2. by rewrite iso_sym; apply iso_output.
           by move=> /eqiso peqm; apply: iso_trans (iso_trans isog1k1 peqm) isog2k2.
+        Qed.
+
+        Lemma iso_can_trans_ts (M : seq (triple I B L) -> seq (triple I B L)) ts1 ts2 (u1 : uniq ts1) (u2 : uniq ts2) (uniq_output : forall ts, uniq ts -> uniq (M ts)) (iso_output : forall ts, uniq ts -> iso_ts ts (M ts)) :
+          iso_ts ts1 ts2 -> iso_ts (M ts1) (M ts2).
+        Proof.
+          have isog1k1 : iso_ts (M ts1) ts1.
+            rewrite iso_ts_sym //; last by apply (uniq_output _).
+            by apply iso_output.
+          have isog2k2 : iso_ts ts2 (M ts2). by apply iso_output.
+          by move=> peqm; apply: (iso_ts_trans (iso_ts_trans isog1k1 peqm) isog2k2).
         Qed.
 
         Lemma iso_can_trans M g1 g2 (iso_output : mapping_is_iso_mapping M) :
@@ -1163,7 +1207,7 @@ Canonical rdf_OrderType (d1 d2 : unit) (I L: orderType d1) (B : orderType d2)
   := Eval hnf in OrderOfChoiceType tt (@rdf_leOrderMixin d1 d2 I L B).
 
 Canonical ts_OPOrderType (d1 d2 : unit) (I L : orderType d1) (B : orderType d2) :=
-  Eval hnf in  Order.Total.porderType (rdf_OrderType I L B).
+  Eval hnf in  Order.Total.porderType (ts_OrderType I L B).
 
 End Rdf.
 
